Progress towards showing the connection between ACL2 and HOL ordinals.
In particular, show that the ord_less from ordinalNotation is the same
as < on the “real” ordinals.

examples/set-theory/hol_sets/ordNotationSemanticsScript.sml
@@ -2,12 +2,21 @@ open HolKernel Parse boolLib bossLib
 
 open ordinalTheory cardinalTheory ordinalNotationTheory
 
+open lcsymtacs
+
 val _ = new_theory "ordNotationSemantics"
+
+val _ = export_rewrites ["ordinalNotation.finp_def", "ordinalNotation.tail_def",
+                         "ordinalNotation.is_ord_equations",
+                         "ordinalNotation.osyntax_size_def",
+                         "ordinalNotation.oless_equations",
+                         "ordinalNotation.expt_def"]
 
 val ordModel_def = Define`
   (ordModel (End n) = &n) ∧
   (ordModel (Plus e c t) = &c * ω ** ordModel e + ordModel t)
 `
+val _ = export_rewrites ["ordModel_def"]
 
 val _ = add_rule {fixity = Closefix, term_name = "ordModel",
                   block_style = (AroundEachPhrase, (PP.CONSISTENT,2)),
@@ -20,6 +29,162 @@ val osyntax_EQ_0 = store_thm(
   Induct_on `is_ord` THEN SRW_TAC [][ordModel_def] THEN
   `k ≠ 0` by DECIDE_TAC THEN SRW_TAC [][ordEXP_EQ_0]);
 
+val CNF_nat = store_thm(
+  "CNF_nat",
+  ``CNF &n = if n = 0 then [] else [(&n,0)]``,
+  rw[] >> match_mp_tac polyform_UNIQUE >> rw[is_polyform_def] >> decide_tac);
+
+(* val ordModel_11 = store_thm(
+  "ordModel_11",
+  ``is_ord m ∧ is_ord n ⇒ ((⟦m⟧ = ⟦n⟧) ⇔ (m = n))``,
+  qsuff_tac `∀m. is_ord m ⇒ ∀n. is_ord n ∧ (⟦m⟧ = ⟦n⟧) ⇒ (m = n)`
+  >- metis_tac[] >> Induct_on `is_ord` >> simp[] >> conj_tac
+  >- (map_every qx_gen_tac [`k`, `n`] >>
+      `(∃k2. n = End k2) ∨ ∃c e t. n = Plus e c t`
+        by (Cases_on `n` >> simp[])
+      >- simp[] >>
+      strip_tac >> rw[] >> fs[] >>
+      `&k < ω` by simp[] >>
+      `ω ≤ ω ** ⟦e⟧`
+        by (simp_tac bool_ss [SimpR ``ordlt``, Once (GSYM ordEXP_1R)] >>
+            match_mp_tac ordEXP_le_MONO_R >> simp[] >> strip_tac >>
+            `⟦e⟧ = 0` by metis_tac [IFF_ZERO_lt] >> metis_tac [osyntax_EQ_0]) >>
+      `ω ** ⟦e⟧ ≤ &c * ω ** ⟦e⟧` by simp[] >>
+      `&c * ω ** ⟦e⟧ ≤ &c * ω ** ⟦e⟧ + ⟦t⟧` by simp[] >>
+      metis_tac [ordlte_TRANS, ordle_TRANS, ordlt_REFL]) >>
+  map_every qx_gen_tac [`e`, `c`, `t`] >> strip_tac
+*)
+
+val oless_0 = store_thm(
+  "oless_0",
+  ``∀n. oless n (End 0) = F``,
+  Cases_on `n` >> simp[]);
+val _ = export_rewrites ["oless_0"]
+
+val oless_0a = store_thm(
+  "oless_0a",
+  ``oless (End 0) n ⇔ n ≠ End 0``,
+  Cases_on `n` >> simp[]);
+val _ = export_rewrites ["oless_0a"]
+
+val oless_x_End = store_thm(
+  "oless_x_End",
+  ``oless x (End n) ⇔ ∃m. (x = End m) ∧ m < n``,
+  Cases_on `x` >> simp[]);
+
+val is_ord_expt = store_thm(
+  "is_ord_expt",
+  ``is_ord e ⇒ is_ord (expt e)``,
+  Cases_on `e` >> simp[]);
+
+val polyform_eval_poly = store_thm(
+  "polyform_eval_poly",
+  ``1 < α ∧ is_polyform α β ⇒ (polyform α (eval_poly α β) = β)``,
+  strip_tac >> match_mp_tac polyform_UNIQUE >> simp[]);
+
+(*
+val notation_exists = store_thm(
+  "notation_exists",
+  ``∀α. α < ε₀ ⇒
+        ∃n. is_ord n ∧ (⟦n⟧ = α) ∧
+            (α ≠ 0 ⇒ (⟦expt n⟧ = SND (HD (CNF α)))) ∧
+            ∀b. is_ord b ⇒ (oless b n ⇔ ⟦b⟧ < α)``,
+  ho_match_mp_tac ord_induction >> rpt strip_tac >>
+  `(CNF α = []) ∨ ∃c e t. (CNF α = (c,e)::t)`
+    by metis_tac [listTheory.list_CASES, pairTheory.pair_CASES]
+  >- (fs[polyform_EQ_NIL] >> qexists_tac `End 0` >> simp[]) >>
+  `(eval_poly ω ((c,e)::t) = α) ∧ is_polyform ω ((c,e)::t)`
+    by metis_tac [polyform_def, fromNat_lt_omega] >>
+  fs[] >>
+  `c < ω ∧ 0 < c ∧ is_polyform ω t`
+    by (imp_res_tac is_polyform_CONS_E >> simp[]) >>
+  `eval_poly ω t < α`
+    by (rw[] >> match_mp_tac ordlte_TRANS >>
+        qexists_tac `ω ** e` >> conj_tac
+        >- (match_mp_tac (GEN_ALL is_polyform_head_dominates_tail) >>
+            metis_tac[fromNat_lt_omega]) >>
+        match_mp_tac ordle_TRANS >> qexists_tac `c * ω ** e` >> simp[] >>
+        qsuff_tac `c ≠ 0` >- simp[] >> strip_tac >> fs[]) >>
+  `∃tn. is_ord tn ∧ (⟦tn⟧ = eval_poly ω t) ∧
+        (eval_poly ω t ≠ 0 ⇒ (⟦expt tn⟧ = SND (HD (CNF (eval_poly ω t))))) ∧
+        ∀b. is_ord b ⇒ (oless b tn ⇔ ⟦b⟧ < eval_poly ω t)`
+    by (first_x_assum (qspec_then `eval_poly ω t` mp_tac) >> simp[] >>
+        disch_then match_mp_tac >> metis_tac [ordlt_TRANS]) >>
+  `∃cn. c = &cn` by metis_tac[lt_omega] >>
+  `e < α`
+    by (spose_not_then strip_assume_tac >>
+        `c * ω ** e ≤ α` by rw[] >>
+        `ω ** e ≤ c * ω ** e` by (simp[] >> qsuff_tac `cn ≠ 0` >- simp[] >>
+                                  strip_tac >> fs[]) >>
+        `ω ** e ≤ e` by metis_tac [ordle_TRANS] >>
+        `ε₀ ≤ e` by metis_tac [epsilon0_least_fixpoint] >>
+        `α < e` by metis_tac [ordlte_TRANS] >>
+        `e ≤ ω ** e` by simp[x_le_ordEXP_x] >>
+        metis_tac [ordlt_REFL, ordlte_TRANS, ordle_TRANS]) >>
+    Cases_on `e = 0`
+    >- (qexists_tac `End cn` >> simp[] >> fs[] >>
+        `&cn = α`
+          by (qsuff_tac `t = []` >- (strip_tac >> fs[]) >>
+              spose_not_then strip_assume_tac >>
+              `∃c' e' t'. t = (c',e')::t'`
+                by metis_tac [listTheory.list_CASES, pairTheory.pair_CASES] >>
+              fs[is_polyform_def]) >>
+        simp[] >> rw[] >> simp[oless_x_End] >> eq_tac >- (rw[] >> rw[]) >>
+        pop_assum mp_tac >>
+        `(∃m. b = End m) ∨ ∃e c t. b = Plus e c t` by (Cases_on `b` >> simp[])
+        >- simp[] >>
+        simp[] >> strip_tac >>
+        match_mp_tac ordle_TRANS >> qexists_tac `ω` >> simp[] >>
+        conj_tac >- simp[ordle_lteq] >>
+        match_mp_tac ordle_TRANS >> qexists_tac `&c * ω ** ⟦e⟧` >> simp[] >>
+        match_mp_tac ordle_TRANS >> qexists_tac `ω ** ⟦e⟧` >> simp[] >>
+        match_mp_tac ordle_TRANS >> qexists_tac `ω ** 1` >> simp[] >>
+        strip_tac >> metis_tac [osyntax_EQ_0, IFF_ZERO_lt]) >>
+    `∃en. is_ord en ∧ (⟦en⟧ = e) ∧
+          ∀b. is_ord b ⇒ (oless b en ⇔ ⟦b⟧ < e)` by metis_tac[ordlt_TRANS] >>
+    `en ≠ End 0` by (strip_tac >> fs[]) >>
+    qexists_tac `Plus en cn tn` >> simp[] >>
+    rpt strip_tac
+    >- (rw[] >> fs[])
+    >- (`(t = []) ∨ ∃c2 e2 t2. t = (c2,e2)::t2`
+          by metis_tac [listTheory.list_CASES, pairTheory.pair_CASES]
+        >- (fs[] >>
+            `tn = End 0` by metis_tac [osyntax_EQ_0] >> fs[] >>
+            metis_tac [IFF_ZERO_lt]) >>
+        `CNF (eval_poly ω t) = t` by simp[polyform_eval_poly] >>
+        pop_assum SUBST_ALL_TAC >>
+        `eval_poly ω t ≠ 0`
+          by (fs[is_polyform_def, ordEXP_EQ_0] >>
+              imp_res_tac is_polyform_CONS_E >> metis_tac [IFF_ZERO_lt]) >>
+        simp[is_ord_expt] >> fs[is_polyform_def])
+    >- rw[] >>
+    `(∃m. b = End m) ∨ (∃e0 c0 t0. b = Plus e0 c0 t0)`
+      by (Cases_on `b` >> simp[])
+    >- (simp[] >> rw[] >>
+        match_mp_tac ordlte_TRANS >> qexists_tac `ω` >> simp[] >>
+        match_mp_tac ordle_TRANS >> qexists_tac `&cn * ω ** ⟦en⟧` >> simp[]>>
+        match_mp_tac ordle_TRANS >> qexists_tac `ω ** ⟦en⟧` >>
+        simp[ordEXP_EQ_0]>> conj_tac
+        >- (match_mp_tac ordle_TRANS >> qexists_tac `ω ** 1` >> simp[] >>
+            metis_tac [IFF_ZERO_lt]) >>
+        fs[] >> decide_tac) >>
+    simp[] >> fs[] >>
+    Cases_on `e0 = en`
+    >- (simp[] >> Cases_on `c0 = cn` >> simp[] >> rw[] >>
+
+
+
+
+
+
+        Cases_on `en` >> fs[]
+        >- (`0 < n` by decide_tac >> simp[oless_rules]) >>
+        simp[oless_rules]) >>
+
+
+*)
+
+
 val ordModel_lt_epsilon0 = store_thm(
   "ordModel_lt_epsilon0",
   ``∀a. ⟦a⟧ < ε₀``,
@@ -27,30 +192,193 @@ val ordModel_lt_epsilon0 = store_thm(
   SRW_TAC [][ordMUL_under_epsilon0, ordEXP_under_epsilon0,
              ordADD_under_epsilon0, ordModel_def]);
 
-(*
+val ordpolyform_def = Define`
+  (ordpolyform (End n) = [(&n:'a ordinal,&0:'a ordinal)]) ∧
+  (ordpolyform (Plus e c t) = (&c,⟦e⟧)::ordpolyform t)
+`;
+val _ = export_rewrites ["ordpolyform_def"]
+
+val ordpolyform_correct = store_thm(
+  "ordpolyform_correct",
+  ``eval_poly ω (ordpolyform e) = ⟦e⟧``,
+  Induct_on `e` >> rw[ordModel_def]);
+
+val asimp = asm_simp_tac (srw_ss() ++ ARITH_ss)
+val dsimp = asm_simp_tac (srw_ss() ++ boolSimps.DNF_ss)
+
 val ord_less_models_ordlt = store_thm(
   "ord_less_models_ordlt",
-  ``∀x y. ord_less x y ⇒ ⟦x⟧ < ⟦y⟧``,
-  SIMP_TAC (srw_ss()) [ord_less_def] THEN
-  completeInduct_on `MAX (osyntax_size x) (osyntax_size y)` THEN
-  FULL_SIMP_TAC (srw_ss() ++ boolSimps.DNF_ss) [] THEN
-  SIMP_TAC (srw_ss()) [Once oless_cases] THEN SRW_TAC [][] THEN
-  SRW_TAC [][ordModel_def] THENL [
-    MATCH_MP_TAC ordlte_TRANS THEN Q.EXISTS_TAC `ω` THEN SRW_TAC [][] THEN
-    MATCH_MP_TAC ordle_TRANS THEN Q.EXISTS_TAC `&k2 * ω ** ⟦e2⟧` THEN
-    SRW_TAC [][] THEN
-    MATCH_MP_TAC ordle_TRANS THEN Q.EXISTS_TAC `ω ** ⟦e2⟧` THEN
-    SRW_TAC [][] THENL [
+  ``∀x. is_ord x ⇒
+        (∀y. oless x y ∧ is_ord y ⇒ ⟦x⟧ :α ordinal < ⟦y⟧) ∧
+        (¬finp x ⇒ ⟦tail x⟧ < ω ** ⟦expt x⟧ :α ordinal)``,
+  completeInduct_on `osyntax_size x` THEN
+  RULE_ASSUM_TAC
+    (SIMP_RULE (srw_ss() ++ boolSimps.DNF_ss) [AND_IMP_INTRO]) >> fs[] >>
+  gen_tac >>
+  `(∃m. x = End m) ∨ (∃e c t. x = Plus e c t)` by (Cases_on `x` >> simp[])
+  >- (simp[] >> strip_tac >> qx_gen_tac `y` >>
+      `(∃n. y = End n) ∨ (∃e c t. y = Plus e c t)` by (Cases_on `y` >> simp[])>>
+      simp[] >> strip_tac >>
+      match_mp_tac ordlte_TRANS >> qexists_tac `ω` >> rw[] >>
+      match_mp_tac ordle_TRANS >> qexists_tac `&c * ω ** ⟦e⟧` >> rw[] >>
+      match_mp_tac ordle_TRANS >> qexists_tac `ω ** ⟦e⟧` >>
+      asm_simp_tac (srw_ss() ++ ARITH_ss) [] >>
       SIMP_TAC bool_ss [Once (GSYM ordEXP_1R), SimpR ``ordlt``] THEN
-      MATCH_MP_TAC ordEXP_le_MONO_R THEN
-      FULL_SIMP_TAC (srw_ss()) [is_ord_equations] THEN
-      STRIP_TAC THEN
-      `⟦e2⟧ = 0` by METIS_TAC [IFF_ZERO_lt] THEN METIS_TAC [osyntax_EQ_0],
-      FULL_SIMP_TAC (srw_ss() ++ ARITH_ss) [is_ord_equations]
-    ],
+      MATCH_MP_TAC ordEXP_le_MONO_R THEN simp[] >>
+      metis_tac [IFF_ZERO_lt, osyntax_EQ_0]) >>
+  simp[] >> disch_then SUBST_ALL_TAC >> strip_tac >>
+  REVERSE conj_tac
+  >- (`ω ** ⟦e⟧ = ⟦Plus e 1 (End 0)⟧` by simp[] >> pop_assum SUBST1_TAC >>
+      first_assum match_mp_tac >> simp[] >> Cases_on `t` >> fs[]) >>
+  qx_gen_tac `y` >>
+  `(∃n. y = End n) ∨ (∃e2 c2 t2. y = Plus e2 c2 t2)`
+    by (Cases_on `y` >> simp[]) >> simp[] >> strip_tac
+  >- (`⟦t⟧ < ⟦Plus e 1 (End 0)⟧`
+        by (first_assum match_mp_tac >> asimp[] >> Cases_on `t` >> fs[]) >>
+      pop_assum mp_tac >> simp[] >> strip_tac >>
+      match_mp_tac ordlt_TRANS >> qexists_tac `&(SUC c) * ω ** ⟦e⟧` >>
+      conj_tac
+      >- (match_mp_tac ordlte_TRANS >>
+          qexists_tac `&c * ω ** ⟦e⟧ + ω ** ⟦e⟧` >> simp[]) >>
+      match_mp_tac ordlte_TRANS >> qexists_tac `ω ** ⟦e2⟧` >> REVERSE conj_tac
+      >- (match_mp_tac ordle_TRANS >> qexists_tac `&c2 * ω ** ⟦e2⟧` >>
+          simp[]) >>
+      `&SUC c * ω ** ⟦e⟧ = eval_poly ω [(&SUC c, ⟦e⟧)]` by simp[] >>
+      pop_assum SUBST1_TAC >>
+      match_mp_tac (GEN_ALL is_polyform_head_dominates_tail) >>
+      simp[is_polyform_def] >> qexists_tac `1` >> simp[])
+  >- (simp[] >>
+      `⟦t⟧ < ⟦Plus e 1 (End 0)⟧`
+        by (first_assum match_mp_tac >> asimp[] >> Cases_on `t` >> fs[]) >>
+      pop_assum mp_tac >> simp[] >> strip_tac >>
+      match_mp_tac ordlte_TRANS >> qexists_tac `&(SUC c) * ω ** ⟦e2⟧` >>
+      conj_tac >- simp[] >>
+      match_mp_tac ordle_TRANS >> qexists_tac `&c2 * ω ** ⟦e2⟧` >> simp[]) >>
+  simp[]);
 
-    FULL_SIMP_TAC (srw_ss()) [is_ord_equations, arithmeticTheory.MAX_LT]
-    ...
+val oless_total = store_thm(
+  "oless_total",
+  ``∀m n. oless m n ∨ oless n m ∨ (m = n)``,
+  Induct
+  >- (map_every qx_gen_tac [`i`, `n`] >>
+      `(∃j. n = End j) ∨ (∃e2 c2 t2. n = Plus e2 c2 t2)`
+        by (Cases_on `n` >> simp[]) >> simp[]) >>
+  map_every qx_gen_tac [`i`, `n`] >>
+  qmatch_abbrev_tac `oless (Plus e1 i t1) n ∨ FOO` >>
+  markerLib.RM_ALL_ABBREVS_TAC >>
+  `(∃j. n = End j) ∨ (∃e2 j t2. n = Plus e2 j t2)`
+    by (Cases_on `n` >> simp[]) >> simp[] >>
+  `oless e1 e2 ∨ oless e2 e1 ∨ (e2 = e1)` by metis_tac[] >> rw[] >>
+  `oless t1 t2 ∨ oless t2 t1 ∨ (t2 = t1)` by metis_tac[] >> rw[] >>
+  metis_tac [DECIDE ``x:num < y ∨ y < x ∨ (x = y)``]);
+
+val ord_less_modelled = store_thm(
+  "ord_less_modelled",
+  ``ord_less x y ⇔ is_ord x ∧ is_ord y ∧ ⟦x⟧ < ⟦y⟧``,
+  metis_tac [ord_less_def, ord_less_models_ordlt, ordlt_REFL, ordlt_TRANS,
+             oless_total])
+
+val oless_modelled = store_thm(
+  "oless_modelled",
+  ``is_ord x ∧ is_ord y ⇒ (oless x y ⇔ ⟦x⟧ < ⟦y⟧)``,
+  metis_tac [ord_less_def, ord_less_modelled]);
+
+(* |- ⟦expt t⟧ < ⟦e⟧ ∧ is_ord e ∧ is_ord t ⇒ ⟦t⟧ < ω ** ⟦e⟧ *)
+val neqend0_lemma = prove(
+  ``x < ⟦e⟧ ⇒ e ≠ End 0``,
+  rpt strip_tac >> fs[]);
+
+val tail_dominated = save_thm(
+  "tail_dominated",
+  ord_less_models_ordlt
+    |> Q.SPEC `Plus e 1 t`
+    |> SIMP_RULE (srw_ss() ++ boolSimps.CONJ_ss)
+                 [oless_modelled, is_ord_expt]
+    |> REWRITE_RULE [neqend0_lemma |> Q.INST [`x` |-> `⟦expt t⟧`] |> UNDISCH]
+    |> REWRITE_RULE [ASSUME ``⟦expt t⟧ < ⟦e⟧ :α ordinal``]
+    |> DISCH_ALL |> REWRITE_RULE [AND_IMP_INTRO]);
+
+val sup_eq_sup = store_thm(
+  "sup_eq_sup",
+  ``(s1:α ordinal set) ≼ univ(:α inf) ∧
+    (s2:α ordinal set) ≼ univ(:α inf) ∧
+    (∀a. a ∈ s1 ⇒ ∃b. b ∈ s2 ∧ a ≤ b) ∧
+    (∀b. b ∈ s2 ⇒ ∃a. a ∈ s1 ∧ b ≤ a) ⇒ (sup s1 = sup s2)``,
+  strip_tac >> match_mp_tac ordle_ANTISYM >> simp[sup_thm] >>
+  metis_tac [suple_thm, ordle_TRANS]);
+
+(*
+val addL_disappears = store_thm(
+  "addL_disappears",
+  ``∀e a. a < ω ** e ⇒ (a + ω ** e = ω ** e)``,
+  ho_match_mp_tac simple_ord_induction >> simp[] >> rpt conj_tac
+  >- (qx_gen_tac `a` >> strip_tac >> `a = 0` by metis_tac [IFF_ZERO_lt] >>
+      simp[])
+  >- (simp[omega_islimit] >> qx_gen_tac `e` >> strip_tac >> qx_gen_tac `a` >>
+      dsimp[sup_thm, IMAGE_cardleq_rwt, preds_inj_univ] >> qx_gen_tac `c` >>
+      strip_tac >>
+      `IMAGE (λy. y * ω ** e) (preds ω) ≠ ∅`
+        by simp[pred_setTheory.EXTENSION] >>
+      simp[ordADD_continuous, IMAGE_cardleq_rwt, preds_inj_univ] >>
+      simp[GSYM pred_setTheory.IMAGE_COMPOSE, combinTheory.o_ABS_R] >>
+      match_mp_tac sup_eq_sup >> dsimp[IMAGE_cardleq_rwt, preds_inj_univ] >>
+      conj_tac
+      >- (qx_gen_tac `d` >>
+          disch_then (Q.X_CHOOSE_THEN `dn` STRIP_ASSUME_TAC o
+                      SIMP_RULE (srw_ss()) [lt_omega]) >>
+          `(dn = 0) ∨ ∃dn0. dn = SUC dn0` by (Cases_on `dn` >> simp[])
+          >- (rw[] >> qexists_tac `c` >> simp[ordle_lteq]) >>
+          rw[]
+
+
+      AP_TERM_TAC >> simp[pred_setTheory.EXTENSION] >>
+      qx_gen_tac `α` >>
+      `0 < c` by (spose_not_then strip_assume_tac >> fs[]) >>
+      `0 < ω ** e` by (spose_not_then strip_assume_tac >> fs[]) >>
+      qspecl_then [`a`, `ω ** e`] mp_tac ordDIVISION >>
+      qabbrev_tac `q = a / ω ** e` >> qabbrev_tac `r = a % ω ** e` >>
+      simp[] >> strip_tac
+
+       0 < k2 ∧ e1 < e2 ⇒
+       (&k1 * ω ** e1 + &k2 * ω ** e2 = &k2 * ω ** e2)``,
+  ho_match_mp_tac simple_ord_induction >> simp[]
+
+val add_nat1_disappears = store_thm(
+  "add_nat1_disappears",
+  ``∀α. ω ≤ α ⇒ (&n + α = α)``,
+  ho_match_mp_tac simple_ord_induction >>
+  simp_tac (srw_ss() ++ boolSimps.CONJ_ss)[AND_IMP_INTRO] >> conj_tac
+  >- (rw[ordle_lteq] >> fs[ordlt_SUC_DISCRETE] >>
+      metis_tac [omega_islimit, islimit_SUC]) >>
+  qx_gen_tac `a` >> strip_tac >>
+  qmatch_abbrev_tac `sup someset = a` >>
+  `someset ≼ univ(:α inf)`
+    by simp[Abbr`someset`, IMAGE_cardleq_rwt, preds_inj_univ] >>
+  `dclose someset = preds (sup someset)` by simp[preds_sup] >>
+  qsuff_tac `dclose someset = preds a` >- (strip_tac >> fs[]) >>
+  dsimp[Abbr`someset`, pred_setTheory.EXTENSION, sup_thm] >>
+  qx_gen_tac `b` >> Cases_on `b < ω`
+  >- (`b < a` by metis_tac [ordlte_TRANS] >> simp[] >>
+      `∃bn. b = &bn` by metis_tac [lt_omega] >> qexists_tac `b^+` >>
+      conj_tac >- metis_tac [islimit_SUC_lt] >> simp[] >>
+      simp_tac (bool_ss ++ ARITH_ss) [GSYM fromNat_SUC, fromNat_ordlt]) >>
+  eq_tac
+  >- (disch_then (Q.X_CHOOSE_THEN `c` strip_assume_tac) >>
+      qsuff_tac `ω ≤ c` >- metis_tac [ordlt_TRANS] >>
+      disch_then (strip_assume_tac o SIMP_RULE (srw_ss()) [lt_omega]) >>
+      fs[] >>
+      metis_tac [fromNat_lt_omega, ordlt_TRANS, ordlt_REFL, ordlte_TRANS]) >>
+  strip_tac >> qexists_tac `b^+` >>
+  `b^+ < a` by metis_tac [islimit_SUC_lt] >> simp[]);
+
+val ord_add_correct = store_thm(
+  "ord_add_correct",
+  ``∀x y. is_ord x ∧ is_ord y ⇒ (⟦ord_add x y⟧ = ⟦x⟧ + ⟦y⟧)``,
+  ho_match_mp_tac ord_add_ind >>
+  simp_tac (srw_ss() ++ boolSimps.CONJ_ss)
+    [ord_add_def, oless_modelled, AND_IMP_INTRO, is_ord_expt, ordADD_ASSOC] >>
+  rw[]
+
+  Cases_on `x` >> Cases_on `y` >> simp[ord_add_def, oless_modelled]
 *)
-
 val _ = export_theory()
